coq/cclc/cclc_linearity.v
@@ -1,10 +1,10 @@
 From mathcomp Require Import ssreflect ssrbool eqtype ssrnat seq.
 From Coq Require Import ssrfun Utf8 Classical.
 Require Import AutosubstSsr ARS 
-  clc_context clc_ast clc_confluence clc_subtype clc_typing
+  clc_context clc_ast clc_confluence clc_subtype clc_dual clc_typing
   clc_weakening clc_substitution clc_inversion clc_validity
   clc_soundness clc_linearity
-  cclc_ast cclc_dual cclc_typing.
+  cclc_ast cclc_typing.
 
 Set Implicit Arguments.
 Unset Strict Implicit.
