coq/cclc/clc_inversion.v
@@ -1,7 +1,7 @@
 From mathcomp Require Import ssreflect ssrbool eqtype ssrnat seq.
 From Coq Require Import ssrfun Utf8 Classical.
 Require Import AutosubstSsr ARS 
-  clc_context clc_ast clc_confluence clc_subtype clc_typing
+  clc_context clc_ast clc_confluence clc_subtype clc_dual clc_typing
   clc_weakening clc_substitution.
 
 Set Implicit Arguments.
@@ -269,6 +269,30 @@ Proof.
   move e:(Ch A)=>n tp. elim: tp A e=>//{Γ B s n}.
   move=>Γ A i k tyA ihA A0 [e]; subst.
   by exists i.
+Qed.
+
+Lemma fork_inv Γ m n T t :
+  Γ ⊢ Fork m n : T : t ->
+  exists Γ1 Γ2 A B C s i,
+    t = L /\
+    Sigma (Ch A) Main L L L <: T /\
+    A ~ B /\
+    Γ1 ∘ Γ2 => Γ /\
+    [Γ1] ⊢ Ch A : L @ i : U /\
+    [Γ2] ⊢ Ch B : L @ i : U /\
+    Γ1 ⊢ m : Main : L /\
+    _: Ch B :L Γ2 ⊢ n : C : s.
+Proof.
+  move e:(Fork m n)=>x tp. elim: tp m n e=>//{Γ x T t}.
+  move=>Γ1 Γ2 Γ m n A B C s i d mrg tyA _ tyB _ tym _ tyn _ m0 n0 [e1 e2]; subst.
+  exists Γ1. exists Γ2. exists A. exists B. exists C. exists s. exists i.
+  repeat split; eauto.
+  move=>Γ A B m s i sb tym ih tyB _ m0 n e; subst.
+  have{ih}[G1[G2[Ax[Bx[Cx[s0[i0 e]]]]]]]:=ih _ _ erefl.
+  firstorder; subst.
+  exists G1. exists G2. exists Ax. exists Bx. exists Cx. exists s0. exists i0.
+  repeat split; eauto.
+  apply: sub_trans; eauto.
 Qed.
 
 Lemma recv_inv Γ m C t :
